WIP

SSA/Core/Framework.lean
@@ -65,39 +65,40 @@ theorem _root_.Pure.pure_cast {f} [inst : Pure f] (b : β) (h : β = α) :
 
 /- # Classes -/
 
-abbrev RegionSignature Ty := List (Ctxt Ty × Ty)
+abbrev RegionSignature Ty := List (Ctxt Ty × List Ty)
 
 structure Signature (Ty : Type) where
   mkEffectful ::
-  sig        : List Ty
-  regSig     : RegionSignature Ty
-  outTy      : Ty
-  effectKind : EffectKind := .pure
+  sig         : List Ty
+  regSig      : RegionSignature Ty
+  returnTypes : List Ty
+  effectKind  : EffectKind := .pure
 
-abbrev Signature.mk (sig : List Ty) (regSig : RegionSignature Ty) (outTy : Ty) : Signature Ty :=
- { sig := sig, regSig := regSig, outTy := outTy }
+abbrev Signature.mk (sig : List Ty) (regSig : RegionSignature Ty) (returnTypes : List Ty) : Signature Ty :=
+ { sig, regSig, returnTypes }
 
 class DialectSignature (d : Dialect) where
   signature : d.Op → Signature d.Ty
 export DialectSignature (signature)
 
-section
+namespace DialectSignature
 variable {d} [s : DialectSignature d]
 
-def DialectSignature.sig        := Signature.sig ∘ s.signature
-def DialectSignature.regSig     := Signature.regSig ∘ s.signature
-def DialectSignature.outTy      := Signature.outTy ∘ s.signature
-def DialectSignature.effectKind := Signature.effectKind ∘ s.signature
+def sig          := Signature.sig ∘ s.signature
+def regSig       := Signature.regSig ∘ s.signature
+def returnTypes  := Signature.returnTypes ∘ s.signature
+def effectKind   := Signature.effectKind ∘ s.signature
 
-end
-
+end DialectSignature
 
 class DialectDenote (d : Dialect) [TyDenote d.Ty] [DialectSignature d] where
   denote : (op : d.Op) → HVector toType (DialectSignature.sig op) →
-    (HVector (fun t : Ctxt d.Ty × d.Ty => t.1.Valuation
-      → EffectKind.impure.toMonad d.m (toType t.2))
+    (HVector (fun t : Ctxt d.Ty × List d.Ty =>
+      t.1.Valuation
+      → EffectKind.impure.toMonad d.m (HVector toType t.2))
             (DialectSignature.regSig op)) →
-    ((DialectSignature.effectKind op).toMonad d.m (toType <| DialectSignature.outTy op))
+    ((DialectSignature.effectKind op).toMonad d.m
+      (HVector toType <| DialectSignature.returnTypes op))
 
 /-
 Some considerations about purity:
@@ -149,34 +150,44 @@ variable (d : Dialect) [DialectSignature d]
 
 mutual
 /-- An intrinsically typed expression whose effect is *at most* EffectKind -/
-inductive Expr : (Γ : Ctxt d.Ty) → (eff : EffectKind) → (ty : d.Ty) → Type where
+inductive Expr : (Γ : Ctxt d.Ty) → (eff : EffectKind) → (ty : List d.Ty) → Type where
   | mk {Γ} {ty} (op : d.Op)
-    (ty_eq : ty = DialectSignature.outTy op)
+    (ty_eq : ty = DialectSignature.returnTypes op)
     (eff_le : DialectSignature.effectKind op ≤ eff)
     (args : HVector (Var Γ) <| DialectSignature.sig op)
     /- For now, assume that regions are impure.
        We keep it this way to minimize the total amount of disruption in our definitions.
        We shall change this once the rest of the file goes through. -/
-    (regArgs : HVector (fun t : Ctxt d.Ty × d.Ty => Com t.1 .impure t.2)
+    (regArgs : HVector (fun t : Ctxt d.Ty × List d.Ty => Com t.1 .impure t.2)
       (DialectSignature.regSig op)) : Expr Γ eff ty
-
 
 /-- A very simple intrinsically typed program: a sequence of let bindings.
 Note that the `EffectKind` is uniform: if a `Com` is `pure`, then the expression
 and its body are pure, and if a `Com` is `impure`, then both the expression and
 the body are impure!
 -/
-inductive Com : Ctxt d.Ty → EffectKind → d.Ty → Type where
-  | ret {eff : EffectKind} (v : Var Γ t) : Com Γ eff t
-  | var (e : Expr Γ eff α) (body : Com (Γ.snoc α) eff β) : Com Γ eff β
+inductive Com : Ctxt d.Ty → EffectKind → List d.Ty → Type where
+  | ret {eff : EffectKind} (vs : HVector Γ.Var tys) : Com Γ eff tys
+  | var (e : Expr Γ eff ty) (body : Com (Γ ++ ty) eff β) : Com Γ eff β
 end
+
+/-! ### `Expr` output context -/
+/-- The context immediately *after* this expression. -/
+abbrev Expr.outContext (_ : Expr d Γ eff ts) : Ctxt d.Ty :=
+  Γ ++ ts
+
+/-! ### Regions -/
+abbrev Regions (regSig : RegionSignature d.Ty) : Type :=
+  HVector (fun t => Com d t.1 .impure t.2) regSig
+
+/-! ### Lets -/
 
 /-- `Lets d Γ_in Γ_out` is a sequence of lets which are well-formed under
 context `Γ_out` and result in context `Γ_in`. -/
 inductive Lets (Γ_in : Ctxt d.Ty) (eff : EffectKind) :
     (Γ_out : Ctxt d.Ty) → Type where
   | nil : Lets Γ_in eff Γ_in
-  | var (body : Lets Γ_in eff Γ_out) (e : Expr d Γ_out eff t) : Lets Γ_in eff (Γ_out.snoc t)
+  | var (body : Lets Γ_in eff Γ_out) (e : Expr d Γ_out eff t) : Lets Γ_in eff e.outContext
 
 /-- `Zipper d Γ_in eff Γ_mid ty` represents a particular position in a program, by storing the
 `Lets` that come before this position separately from the `Com` that represents the rest.
@@ -185,11 +196,11 @@ current position.
 
 While technically the position is in between two let-bindings, by convention we say that the first
 binding of `top : Lets ..` is the current binding of a particular zipper. -/
-structure Zipper (Γ_in : Ctxt d.Ty) (eff : EffectKind) (Γ_mid : Ctxt d.Ty) (ty : d.Ty) where
+structure Zipper (Γ_in : Ctxt d.Ty) (eff : EffectKind) (Γ_mid : Ctxt d.Ty) (tys : List d.Ty) where
   /-- The let-bindings at the top of the zipper -/
   top : Lets d Γ_in eff Γ_mid
   /-- The program at the bottom of the zipper -/
-  bot : Com d Γ_mid eff ty
+  bot : Com d Γ_mid eff tys
 
 
 
@@ -228,7 +239,7 @@ private def formatFormalArgListTuple [Repr Ty] (ts : List Ty) : Format :=
 
 mutual
   /-- Convert a HVector of region arguments into a List of format strings. -/
-  partial def reprRegArgsAux [Repr d.Ty] {ts : List (Ctxt d.Ty × d.Ty)}
+  partial def reprRegArgsAux [Repr d.Ty] {ts : RegionSignature d.Ty}
     (regArgs : HVector (fun t => Com d t.1 EffectKind.impure t.2) ts) : List Format :=
     match ts with
     | [] => []
@@ -241,10 +252,10 @@ mutual
 
   partial def Expr.repr (_ : Nat) : Expr d Γ eff t → Format
     | ⟨op, _, _, args, regArgs⟩ =>
-        let outTy := DialectSignature.outTy op
+        let returnTypes := DialectSignature.returnTypes op
         let argTys := DialectSignature.sig op
         let regArgs := Format.parenIfNonempty " (" ")" Format.line (reprRegArgsAux regArgs)
-        f!"{repr op}{formatArgTuple args}{regArgs} : {formatTypeTuple argTys} → ({repr outTy})"
+        f!"{repr op}{formatArgTuple args}{regArgs} : {formatTypeTuple argTys} → ({repr returnTypes})"
 
   /-- Format string for a Com, with the region parentheses and formal argument list. -/
   partial def Com.repr (prec : Nat) (com : Com d Γ eff t) : Format :=
@@ -294,9 +305,9 @@ their types, and the resulting output type.
 -/
 partial def Expr.toString [ToString d.Op] : Expr d Γ eff t → String
   | Expr.mk (op : d.Op) _ _ args _regArgs =>
-    let outTy : d.Ty := DialectSignature.outTy op
+    let returnTypes := DialectSignature.returnTypes op
     let argTys := DialectSignature.sig op
-    s!"{ToString.toString op}{formatArgTuple args} : {formatTypeTupleToString argTys} -> ({ToString.toString outTy})"
+    s!"{ToString.toString op}{formatArgTuple args} : {formatTypeTupleToString argTys} -> ({ToString.toString returnTypes})"
 
 /-- This function recursivly converts the body of a `Com` into its string representation.
 Each bound variable is printed with its index and corresponding expression. -/
@@ -325,7 +336,7 @@ mutual -- DecEq
 variable {d} [DialectSignature d]
 
 protected instance HVector.decidableEqReg [DecidableEq d.Op] [DecidableEq d.Ty] :
-    ∀ {l : List (Ctxt d.Ty × d.Ty)}, DecidableEq (HVector (fun t => Com d t.1 .impure t.2) l)
+    ∀ {l : RegionSignature d.Ty}, DecidableEq (HVector (fun t => Com d t.1 .impure t.2) l)
   | _, .nil, .nil => isTrue rfl
   | _, .cons x₁ v₁, .cons x₂ v₂ =>
     letI := HVector.decidableEqReg v₁ v₂
@@ -333,10 +344,9 @@ protected instance HVector.decidableEqReg [DecidableEq d.Op] [DecidableEq d.Ty] 
     decidable_of_iff (x₁ = x₂ ∧ v₁ = v₂) (by simp)
 
 protected instance Expr.decidableEq [DecidableEq d.Op] [DecidableEq d.Ty] :
-    {Γ : Ctxt d.Ty} → {ty : d.Ty} → DecidableEq (Expr d Γ eff ty)
-  | _, _, .mk op₁ rfl eff_le₁ arg₁ regArgs₁, .mk op₂ eq eff_le₂ arg₂ regArgs₂ =>
-    if ho : op₁ = op₂
-    then by
+    {Γ : Ctxt d.Ty} → {ty : List d.Ty} → DecidableEq (Expr d Γ eff ty)
+  | Γ, _, .mk op₁ rfl eff_le₁ arg₁ regArgs₁, .mk op₂ eq eff_le₂ arg₂ regArgs₂ =>
+    if ho : op₁ = op₂ then by
       subst ho
       letI := HVector.decidableEq arg₁ arg₂
       letI := HVector.decidableEqReg regArgs₁ regArgs₂
@@ -344,10 +354,10 @@ protected instance Expr.decidableEq [DecidableEq d.Op] [DecidableEq d.Ty] :
     else isFalse (by simp_all)
 
 protected instance Com.decidableEq [DecidableEq d.Op] [DecidableEq d.Ty]
-    {Γ : Ctxt d.Ty} {eff : EffectKind} {ty : d.Ty} : DecidableEq (Com d Γ eff ty)
+    {Γ : Ctxt d.Ty} {eff : EffectKind} {tys : List d.Ty} : DecidableEq (Com d Γ eff tys)
   | .ret v₁, .ret v₂ => decidable_of_iff (v₁ = v₂) (by simp)
-  | .var (α := α₁) e₁ body₁, .var (α := α₂) e₂ body₂ =>
-    if hα : α₁ = α₂
+  | .var (ty := ty₁) e₁ body₁, .var (ty := ty₂) e₂ body₂ =>
+    if hα : ty₁ = ty₂
     then by
       subst hα
       letI := Expr.decidableEq e₁ e₂
@@ -367,15 +377,6 @@ end DataStructures
 
 variable {d : Dialect} [DialectSignature d]
 
-
-/-!
-### `Expr` output context
--/
-
-/-- The context immediately *after* this expression. -/
-abbrev Expr.outContext (_ : Expr d Γ eff t) : Ctxt d.Ty :=
-  Γ.snoc t
-
 /-!
 ### Com recursors
 -/
@@ -392,6 +393,11 @@ def Com.recAux' {Γ} : (com : Com d Γ eff t) → motive com
   | Com.ret v => ret v
   | Com.var e body => var e body (Com.recAux' body)
 
+/--
+`Com.rec'` is a simple recursor for `Com` -- meaning it does not facilitate
+mutual recursion on the contained expressions or regions. In return, it has
+nicer def-eqs than a pattern-match based definition would.
+-/
 @[implemented_by Com.recAux', elab_as_elim, induction_eliminator]
 -- ^^^^ `Com.rec` is noncomputable, so have a computable version as well
 --      See `Com.recAux'_eq` for a theorem that states these definitions are equal
@@ -450,43 +456,44 @@ def Com.recPure {t} {motive : ∀ {Γ t}, Com d Γ .pure t → Sort u}
     {Γ} (com : Com d Γ .pure t) : motive com :=
   com.rec' (motive := motive) ret var
 
-def Expr.op {Γ : Ctxt d.Ty} {eff : EffectKind} {ty : d.Ty} (e : Expr d Γ eff ty) : d.Op :=
+def Expr.op {Γ : Ctxt d.Ty} {eff : EffectKind} {ty} (e : Expr d Γ eff ty) : d.Op :=
   Expr.casesOn e (fun op _ _ _ _ => op)
 
-theorem Expr.eff_le {Γ : Ctxt d.Ty} {ty : d.Ty} (e : Expr d Γ eff ty) :
+theorem Expr.eff_le {Γ : Ctxt d.Ty} {ty} (e : Expr d Γ eff ty) :
   DialectSignature.effectKind e.op ≤ eff :=
   Expr.casesOn e (fun _ _ eff_le _ _ => eff_le)
 
-theorem Expr.ty_eq {Γ : Ctxt d.Ty} {ty : d.Ty} (e : Expr d Γ eff ty) :
-    ty = DialectSignature.outTy e.op :=
+theorem Expr.ty_eq {Γ : Ctxt d.Ty} {tys : List d.Ty} (e : Expr d Γ eff tys) :
+    tys = DialectSignature.returnTypes e.op :=
   Expr.casesOn e (fun _ ty_eq _ _ _ => ty_eq)
 
-def Expr.args {Γ : Ctxt d.Ty} {ty : d.Ty} (e : Expr d Γ eff ty) :
+def Expr.args {Γ ts} (e : Expr d Γ eff ts) :
     HVector (Var Γ) (DialectSignature.sig e.op) :=
   Expr.casesOn e (fun _ _ _ args _ => args)
 
-def Expr.regArgs {Γ : Ctxt d.Ty} {ty : d.Ty} (e : Expr d Γ eff ty) :
-    HVector (fun t : Ctxt d.Ty × d.Ty => Com d t.1 .impure t.2) (DialectSignature.regSig e.op) :=
+def Expr.regArgs {Γ ts} (e : Expr d Γ eff ts) :
+    Regions d (DialectSignature.regSig e.op) :=
   Expr.casesOn e (fun _ _ _ _ regArgs => regArgs)
 
 /-! Projection equations for `Expr` -/
 @[simp]
-theorem Expr.op_mk {Γ : Ctxt d.Ty} {ty : d.Ty} {eff : EffectKind} (op : d.Op)
-    (ty_eq : ty = DialectSignature.outTy op)
+theorem Expr.op_mk {Γ : Ctxt d.Ty} {ty} {eff : EffectKind} (op : d.Op)
+    (ty_eq : ty = DialectSignature.returnTypes op)
     (eff_le : DialectSignature.effectKind op ≤ eff)
-    (args : HVector (Var Γ) (DialectSignature.sig op)) (regArgs):
+    (args : HVector (Var Γ) (DialectSignature.sig op))
+    (regArgs) :
     (Expr.mk op ty_eq eff_le args regArgs).op = op := rfl
 
 @[simp]
-theorem Expr.args_mk {Γ : Ctxt d.Ty} {ty : d.Ty} {eff : EffectKind} (op : d.Op)
-    (ty_eq : ty = DialectSignature.outTy op)
+theorem Expr.args_mk {Γ : Ctxt d.Ty} {ty eff op}
+    (ty_eq : ty = DialectSignature.returnTypes op)
     (eff_le : DialectSignature.effectKind op ≤ eff)
     (args : HVector (Var Γ) (DialectSignature.sig op)) (regArgs) :
     (Expr.mk op ty_eq eff_le args regArgs).args = args := rfl
 
 @[simp]
-theorem Expr.regArgs_mk {Γ : Ctxt d.Ty} {ty : d.Ty} {eff : EffectKind} (op : d.Op)
-    (ty_eq : ty = DialectSignature.outTy op)
+theorem Expr.regArgs_mk {Γ : Ctxt d.Ty} {ty eff op}
+    (ty_eq : ty = DialectSignature.returnTypes op)
     (eff_le : DialectSignature.effectKind op ≤ eff)
     (args : HVector (Var Γ) (DialectSignature.sig op)) (regArgs) :
     (Expr.mk op ty_eq eff_le args regArgs).regArgs = regArgs := rfl
@@ -501,10 +508,39 @@ def Com.size : Com d Γ eff t → Nat :=
     /- ret _ -/       (fun _ => 0)
     /- var _ body -/ (fun _ _body bodySize => bodySize + 1)
 
-section Lemmas
+@[grind] def Expr.bvars (e : Expr d Γ eff Δ) : Nat :=
+  (DialectSignature.returnTypes e.op).length
 
-@[simp] lemma Com.size_ret  : (ret v : Com d Γ eff t).size = 0 := rfl
-@[simp] lemma Com.size_var : (var e body : Com d Γ eff t).size = body.size + 1 := rfl
+/-- The number of variables bound in a `Com`. This is related to the `size`, but
+will differ in the presence of let-bindings with multiple return variables.
+
+NOTE: this ignores any regions. -/
+private def Com.bvars : Com d Γ eff t → Nat :=
+  Com.rec'
+    /- ret _ -/      (fun _ => 0)
+    /- var e body -/ (fun e _body bodySize => e.bvars + bodySize)
+
+section Lemmas
+namespace Com
+
+@[simp] lemma size_ret  : (ret v : Com d Γ eff t).size = 0 := rfl
+@[simp] lemma size_var : (var e body : Com d Γ eff t).size = body.size + 1 := rfl
+
+@[simp] lemma bvars_ret  : (ret v : Com d Γ eff t).bvars = 0 := rfl
+@[simp] lemma bvars_var  :
+  (var e body : Com d Γ eff t).bvars = e.bvars + body.bvars := rfl
+
+end Com
+
+/-- Note: the context being accessed (`Γ_out`) is the return context of `e`! -/
+@[simp] lemma Ctxt.get_add_bvars (e : Expr d Γ eff ts) (i : Nat) :
+    e.outContext[i + e.bvars]? = Γ[i]? := by
+  stop
+  rcases e with ⟨op, rfl, _, _⟩
+  rcases Γ_in
+  simp only [get?, instAppend, ofList_append, Expr.bvars, Expr.op_mk, getElem?_ofList]
+  rw [List.getElem?_append_right (by simp)]
+  simp
 
 end Lemmas
 
@@ -514,52 +550,62 @@ end Lemmas
 
 /-- The `outContext` of a program is a context which includes variables for all let-bindings
 of the program. That is, it is the context under which the return value is typed -/
-def Com.outContext {Γ} : Com d Γ eff t → Ctxt d.Ty :=
+def Com.outContext {Γ} : Com d Γ eff ts → Ctxt d.Ty :=
   Com.rec' (motive := fun _ => Ctxt d.Ty)
     (@fun Γ _ => Γ) -- `Com.ret` case
     (fun _ _ r => r) -- `Com.var` case
 
 /-- The difference between the context `Γ` under which `com` is typed, and the output context of
 that same `com` -/
-def Com.outContextDiff (com : Com d Γ eff t) : Γ.Diff com.outContext :=
-  ⟨com.size, by
+def Com.outContextDiff (com : Com d Γ eff ts) : Γ.Diff com.outContext :=
+  ⟨com.bvars, by
     intro i t h;
     unfold outContext
     induction com generalizing i
     case ret => exact h
-    case var ih =>
-      rw [rec'_var, size_var, ← Nat.add_assoc, Nat.add_comm _ 1, ← Nat.add_assoc, ih]
-      simpa [Ctxt.snoc, Nat.add_comm 1 _] using h⟩
+    case var Γ Δ _ _ e _ ih =>
+      simp only [rec'_var, bvars_var]
+      rw [← Nat.add_assoc]
+      apply ih
+      rw [Ctxt.get_add_bvars e, h]⟩
 
 /-- `com.outContextHom` is the canonical homorphism from free variables of `com` to those same
 variables in the output context of `com` -/
 def Com.outContextHom (com : Com d Γ eff t) : Γ.Hom com.outContext :=
   com.outContextDiff.toHom
 
-/-- The return variable of a program -/
-def Com.returnVar : (com : Com d Γ eff t) → Var com.outContext t
-  | .ret v => v
-  | .var _ body => body.returnVar
+/-- The return variables of a program -/
+def Com.returnVars : (com : Com d Γ eff ts) → HVector (Var com.outContext) ts
+  | .ret vs => vs
+  | .var _ body => body.returnVars
+
+/-- The return variable of a program with exactly one return. -/
+def Com.returnVar (com : Com d Γ eff [t]) : Var com.outContext t :=
+  com.returnVars.get (0 : Fin 1)
+
+@[simp] def Expr.contextHom (e : Expr d Γ eff ts) : Γ.Hom e.outContext :=
+  @fun _ => Var.appendInl
 
 section Lemmas
 
-@[simp] lemma Com.outContext_ret (v : Var Γ t) : (ret v : Com d Γ eff t).outContext = Γ := rfl
-@[simp] lemma Com.outContext_var {eff} (e : Expr d Γ eff t) (body : Com d (e.outContext) eff u) :
+@[simp] lemma Com.outContext_ret (vs : HVector Γ.Var t) : (ret vs : Com d Γ eff t).outContext = Γ := rfl
+@[simp] lemma Com.outContext_var {eff} (e : Expr d Γ eff t) (body : Com d e.outContext eff u) :
     (Com.var e body).outContext = body.outContext := rfl
 
-@[simp] lemma Com.outContextHom_ret (v : Var Γ t) :
+@[simp] lemma Com.outContextHom_ret (v : HVector Γ.Var t) :
     (ret v : Com d Γ eff t).outContextHom = Ctxt.Hom.id := rfl
 @[simp] lemma Com.outContextHom_var :
-    (var e body : Com d Γ eff t).outContextHom = body.outContextHom.unSnoc := by
-  funext t' v'
-  simp only [outContext_var, outContextHom, Ctxt.Diff.toHom, Ctxt.Diff.Valid, outContextDiff,
-    size_var, Ctxt.Hom.unSnoc, Var.val_toSnoc]
-  ac_rfl
+    (var e body : Com d Γ eff t).outContextHom
+    = e.contextHom.comp body.outContextHom := by
+  funext t v
+  apply Subtype.eq
+  simp [outContextHom, outContextDiff, Expr.contextHom, Ctxt.Hom.comp, Expr.bvars,
+    e.ty_eq]
+  omega
 
-@[simp] lemma Com.returnVar_ret : returnVar (ret v : Com d Γ eff t) = v := by simp [returnVar]
+@[simp] lemma Com.returnVar_ret : returnVars (ret vs : Com d Γ eff t) = vs := rfl
 @[simp] lemma Com.returnVar_var :
-    returnVar (var (d:=d) (eff:=eff) e body) = body.returnVar := by
-  simp [returnVar]
+    returnVars (var (d:=d) (eff:=eff) e body) = body.returnVars := rfl
 
 end Lemmas
 
@@ -597,21 +643,22 @@ variable [TyDenote d.Ty] [DialectDenote d] [DecidableEq d.Ty] [Monad d.m] [Lawfu
 mutual
 
 def HVector.denote :
-    {l : List (Ctxt d.Ty × d.Ty)} → (T : HVector (fun t => Com d t.1 .impure t.2) l) →
-    HVector (fun t => t.1.Valuation → EffectKind.impure.toMonad d.m (toType t.2)) l
+    {l : RegionSignature d.Ty} → (T : HVector (fun t => Com d t.1 .impure t.2) l) →
+    HVector (fun t => t.1.Valuation → EffectKind.impure.toMonad d.m (HVector toType t.2)) l
   | _, .nil => HVector.nil
   | _, .cons v vs => HVector.cons (v.denote) (HVector.denote vs)
 
-def Expr.denote {ty : d.Ty} (e : Expr d Γ eff ty) (V : Valuation Γ) :
+def Expr.denote {ty} (e : Expr d Γ eff ty) (V : Valuation Γ) :
     eff.toMonad d.m (e.outContext.Valuation) :=
   match e with
   | ⟨op, ty_eq, heff, args, regArgs⟩ => do
       let argsDenote := args.map V
       let val ← EffectKind.liftEffect heff <| DialectDenote.denote op argsDenote regArgs.denote
-      return (V.snoc val).cast (by rw [← ty_eq])
+      return (V ++ val).cast (by rw [← ty_eq])
 
-def Com.denote : Com d Γ eff ty → (Γv : Valuation Γ) → eff.toMonad d.m (toType ty)
-  | .ret e, Γv     => pure (Γv e)
+def Com.denote : Com d Γ eff ty → (Γv : Valuation Γ) →
+    eff.toMonad d.m (HVector toType ty)
+  | .ret vs, Γv     => pure (vs.map Γv)
   | .var e body, V => e.denote V >>= body.denote
 end
 
@@ -643,8 +690,8 @@ the congruence, you can do: `rw [← Lets.denotePure]; congr`
 
 /-- The denotation of a zipper is a composition of the denotations of the constituent
 `Lets` and `Com` -/
-def Zipper.denote (zip : Zipper d Γ_in eff Γ_out ty) (V_in : Valuation Γ_in) :
-    eff.toMonad d.m ⟦ty⟧ :=
+def Zipper.denote (zip : Zipper d Γ_in eff Γ_out tys) (V_in : Valuation Γ_in) :
+    eff.toMonad d.m (HVector toType tys) :=
   (zip.top.denote V_in) >>= zip.bot.denote
 
 section Unfoldings
@@ -653,7 +700,8 @@ open EffectKind (liftEffect)
 
 omit [LawfulMonad d.m] in
 /-- Returns only the result of the current expression. -/
-def Expr.denoteOp (e : Expr d Γ eff ty) (V : Γ.Valuation) : eff.toMonad d.m ⟦ty⟧ :=
+def Expr.denoteOp (e : Expr d Γ eff ty) (V : Γ.Valuation) :
+    eff.toMonad d.m (HVector toType ty) :=
   EffectKind.liftEffect e.eff_le <| cast (by rw [← e.ty_eq]) <|
     DialectDenote.denote e.op (e.args.map V) e.regArgs.denote
 
@@ -669,7 +717,7 @@ Unfortunately, if we define `Expr.denote` in terms of the projections directly,
 the termination checker fails to prove termination. Hence, this workaround.
 -/
 theorem Expr.denote_unfold (e : Expr d Γ eff ty) :
-    e.denote = fun V => V.snoc <$> (e.denoteOp V) := by
+    e.denote = fun V => (V ++ ·) <$> (e.denoteOp V) := by
   rcases e with ⟨op, rfl, _⟩
   simp [denote, denoteOp]
 
@@ -716,22 +764,23 @@ end Unfoldings
 section Lemmas
 
 @[simp] lemma Expr.comap_denote_snocRight (e : Expr d Γ .pure ty) (V : Γ.Valuation) :
-    (Valuation.comap (e.denote V) Hom.id.snocRight) = V := by
+    (Valuation.comap (e.denote V) e.contextHom) = V := by
+  stop
   funext t v; simp [Expr.denote_unfold]; rfl
 
 @[simp] lemma HVector.denote_nil
-    (T : HVector (fun (t : Ctxt d.Ty × d.Ty) => Com d t.1 .impure t.2) []) :
+    (T : HVector (fun (t : Ctxt d.Ty × List d.Ty) => Com d t.1 .impure t.2) []) :
     HVector.denote T = HVector.nil := by
-  cases T; simp [HVector.denote]
+  cases T; rfl
 
 @[simp] lemma HVector.denote_cons
-    (t : Ctxt d.Ty × d.Ty) (ts : List (Ctxt d.Ty × d.Ty))
-    (a : Com d t.1 .impure t.2) (as : HVector (fun t => Com d t.1 .impure t.2) ts) :
-    HVector.denote (.cons a as) = .cons (a.denote) (as.denote) := by
-  simp [HVector.denote]
+    {t : _ × _} {ts : RegionSignature _}
+    (a : Com d t.1 .impure t.2) (as : Regions _ ts) :
+    HVector.denote (.cons a as) = .cons (a.denote) (as.denote) :=
+  rfl
 
-@[simp] lemma Com.denote_ret {eff : EffectKind} (Γ : Ctxt d.Ty) (x : Γ.Var t) :
-    (Com.ret x : Com d Γ eff t).denote = fun Γv => return (Γv x) := by
+@[simp] lemma Com.denote_ret {eff : EffectKind} (Γ : Ctxt d.Ty) (vs : HVector Γ.Var ts) :
+    (Com.ret (eff := eff) vs).denote = fun V => pure (vs.map V) :=
   rfl
 
 @[simp] lemma Com.denote_var [LawfulMonad d.m] {e : Expr d Γ eff α} :
@@ -784,6 +833,7 @@ variable [DialectHRefinement d d]
 /-
 TODO: do we need refinement of expressions? If we do, we need to start by
 defining refinement of (monadic!) Valuations, which will require some more reworking.
+See also the TODO note in Refinement.lean
 -/
 
 -- /--
@@ -800,7 +850,8 @@ respective denotations under every valuation are in the refinement relation.
 -/
 instance : HRefinement (Com d Γ eff₁ t) (Com d Γ eff₂ t) where
   IsRefinedBy c₁ c₂ :=
-    ∀ V, c₁.denote V ⊑ c₂.denote V
+    ∀ V (i : _),
+      (·.get i) <$> c₁.denote V ⊑ (·.get i) <$> c₂.denote V
 
 end Refinement
 
@@ -810,16 +861,16 @@ Map a context homomorphism over a `Expr`/`Com`.
 That is, substitute variables.
 -/
 
-def Expr.changeVars (varsMap : Γ.Hom Γ') {ty : d.Ty} (e : Expr d Γ eff ty) :
+def Expr.changeVars (varsMap : Γ.Hom Γ') {ty} (e : Expr d Γ eff ty) :
     Expr d Γ' eff ty :=
   ⟨e.op, e.ty_eq, e.eff_le, e.args.map varsMap, e.regArgs⟩
 
 def Com.changeVars : Com d Γ eff ty →
     (varsMap : Γ.Hom Γ') →
     Com d Γ' eff ty
-  |  .ret e => fun varsMap => .ret (varsMap e)
+  |  .ret e => fun varsMap => .ret (e.map varsMap)
   |  .var e body => fun varsMap => .var (e.changeVars varsMap)
-      (body.changeVars (fun _ v => varsMap.snocMap v))
+      (body.changeVars (fun _ v => varsMap.append v))
 
 /-! simp-lemmas about `changeVars`-/
 section Lemmas
@@ -839,20 +890,21 @@ variable {Γ Γ' : Ctxt d.Ty} {t} (f : Γ.Hom Γ') (e : Expr d Γ eff t) (V : Γ
     (V : Γ'.Valuation)
     (f : e.outContext.Valuation → eff.toMonad d.m α) :
     (Expr.changeVars varsMap e).denote V
-      >>= (f <| Valuation.comap · varsMap.snocMap)
+      >>= (f <| Valuation.comap · varsMap.append)
     = e.denote (V.comap varsMap) >>= f := by
   simp [denote_unfold]
 
 end Lemmas
 
-@[simp] lemma Com.changeVars_ret (v : Var Γ t) :
-    (Com.ret (d:=d) (eff := eff) v).changeVars = fun (map : Γ.Hom Δ) => Com.ret (map v) := by
+@[simp] lemma Com.changeVars_ret :
+    (Com.ret (d:=d) (Γ:=Γ) (eff := eff) vs).changeVars
+    = fun (map : Γ.Hom Δ) => Com.ret (vs.map map) := by
   funext map
   simp [changeVars]
 
 @[simp] lemma Com.changeVars_var (e : Expr d Γ eff t) (body : Com d _ eff u) :
     (Com.var e body).changeVars
-    = fun (map : Γ.Hom Δ) => Com.var (e.changeVars map) (body.changeVars map.snocMap) := by
+    = fun (map : Γ.Hom Δ) => Com.var (e.changeVars map) (body.changeVars map.append) := by
   simp [changeVars]
 
 -- TODO: this is implied by simpler simp-lemmas, do we need it?
@@ -864,7 +916,7 @@ end Lemmas
     (c.changeVars varsMap).denote =
     fun V => c.denote (V.comap varsMap) := by
   induction c using Com.rec' generalizing Γ' with
-  | ret x      => simp
+  | ret x      => simp [HVector.map_map]; rfl
   | var _ _ ih => simp [denote, ih]
 
 @[simp] lemma Com.denote_changeVars' (varsMap : Γ.Hom Γ') (c : Com d Γ eff ty) :
@@ -875,10 +927,10 @@ end Lemmas
     {c : Com d Γ eff ty} → Ctxt.Hom (outContext (changeVars c map)) (outContext c)
   | .ret _        => cast (by simp) map_inv
   | .var _ body  => cast (by simp) <|
-      Com.outContext_changeVars_hom (map := map.snocMap) map_inv.snocMap (c := body)
+      Com.outContext_changeVars_hom (map := map.append) map_inv.append (c := body)
 
-@[simp] lemma Com.denoteLets_returnVar_pure (c : Com d Γ .pure ty) (Γv : Valuation Γ) :
-    c.denoteLets Γv c.returnVar = c.denote Γv := by
+@[simp] lemma Com.denoteLets_returnVar_pure (c : Com d Γ .pure [ty]) (Γv : Valuation Γ) :
+    c.denoteLets Γv c.returnVar = (c.denote Γv).get (0 : Fin 1) := by
   induction c using Com.rec'
   · simp; rfl
   · rename_i a
